# [Dominanzgesetz](https://de.wikibooks.org/wiki/Formelsammlung_Mathematik:_Logik)

#S-6

> Auch bekannt als Extremalgesetz

## Konjunktion-Form

$A \cdot 0 = 0$  #S-6K

### Beweis S-6K

$A \cdot 0 = A \cdot 0 + 0$  #A-3

$A \cdot 0 + 0 = A \cdot 0 + A \cdot \bar A$  #A-4

$A \cdot 0 + A \cdot \bar A = A \cdot (0 + \bar A)$  #A-2

$A \cdot (0 + \bar A) = A \cdot (\bar A + 0)$  #A-1

$A \cdot (\bar A + 0) = A \cdot \bar A$  #A-3

$A \cdot \bar A = 0$  #A-4

## Disjunktion-Form

$A + 1 = 1$  #S-6D

### Beweis S-6D

$A + 1 = (A + 1) \cdot 1$  #A-3

$(A + 1) \cdot 1 = (A + 1) \cdot (A + \bar A)$  #A-4

$(A + 1) \cdot (A + \bar A) = A + 1 \cdot \bar A$  #A-2

$A + 1 \cdot \bar A = A + \bar A \cdot 1$  #A-1

$A + \bar A \cdot 1 = A + \bar A$  #A-3

$A + \bar A = 1$  #A-4

