# Absorptionsgesetz

#S-7

## Konjunktion-Form

$A \cdot (A + B) = A$  #S-7K

### Beweis S-7K

$A \cdot (A + B) = (A + 0) \cdot (A + B)$  #A-3

$(A + 0) \cdot (A + B) = A + 0 \cdot B$  #A-2

$A + 0 \cdot B = A + B \cdot 0$  #A-1

$A + B \cdot 0 = A + 0$  #S-6

$A + 0= A$  #A-3

## Disjunktion-Form

$A + A \cdot B = A$  #S-7D

### Beweis S-7D

$A + A \cdot B = A \cdot 1 + A \cdot B$  #A-3

$A \cdot 1 + A \cdot B = A \cdot (1 + B)$  #A-2

$A \cdot (1 + B) = A \cdot (B + 1)$  #A-1

$A \cdot (B + 1) = A \cdot 1$  #S-6

$A \cdot 1 = A$  #A-3

