# Doppelte Negation

#S-9

$$\bar{\bar A} = A$$

## Beweis S-9

$\bar{\bar A} = \bar{\bar A} + 0$  #A-3

$\bar{\bar A} + 0 = \bar{\bar A} + A \cdot \bar A$  #A-4

$\bar{\bar A} + A \cdot \bar A = (\bar{\bar A} + A) \cdot (\bar{\bar A} + \bar A)$  #A-2

$(\bar{\bar A} + A) \cdot (\bar{\bar A} + \bar A) = (\bar{\bar A} + A) \cdot (\bar A + \bar{\bar A})$  #A-1

$(\bar{\bar A} + A) \cdot (\bar A + \bar{\bar A}) = (\bar{\bar A} + A) \cdot 1$  #A-4

$(\bar{\bar A} + A) \cdot 1 = \bar{\bar A} + A$  #A-4

$\bar{\bar A} + A = A + \bar{\bar A}$  #A-1

$A + \bar{\bar A} = (A + \bar{\bar A}) \cdot 1$  #A-3

$(A + \bar{\bar A}) \cdot 1 = (A + \bar{\bar A}) \cdot (A + \bar A)$  #A-3

$(A + \bar{\bar A}) \cdot (A + \bar A) = A + \bar{\bar A} \cdot \bar A$  #A-2

$A + \bar{\bar A} \cdot \bar A = A + \bar A \cdot \bar{\bar A}$  #A-1

$A + \bar A \cdot \bar{\bar A} = A + 0$  #A-4

$A + 0 = A$  #A-3

## Noch ein Beweis

$\bar{\bar A} = \bar{\bar A} \cdot 1$  #A-3

$\bar{\bar A} \cdot 1 = \bar{\bar A} \cdot (A + \bar A)$  #A-4

$\bar{\bar A} \cdot (A + \bar A) = \bar{\bar A} \cdot A + \bar{\bar A} \cdot \bar A$  #A-2

$\bar{\bar A} \cdot A + \bar{\bar A} \cdot \bar A = \bar{\bar A} \cdot A + \bar A \cdot \bar{\bar A}$  #A-1

$\bar{\bar A} \cdot A + \bar A \cdot \bar{\bar A} = \bar{\bar A} \cdot A + 0$  #A-4

$\bar{\bar A} \cdot A + 0 = \bar{\bar A} \cdot A$  #A-3

$\bar{\bar A} \cdot A = A \cdot \bar{\bar A}$  #A-1

$A \cdot \bar{\bar A} = A \cdot \bar{\bar A} + 0$  #A-3

$A \cdot \bar{\bar A} + 0 = A \cdot \bar{\bar A} + A \cdot \bar A$  #A-4

$A \cdot \bar{\bar A} + A \cdot \bar A = A \cdot (\bar{\bar A} + \bar A)$  #A-2

$A \cdot (\bar{\bar A} + \bar A) = A \cdot (\bar A + \bar{\bar A})$  #A-1

$A \cdot (\bar A + \bar{\bar A}) = A \cdot 1$  #A-4

$A \cdot 1 = A$  #A-3

